Adding example 4 triggered some bugs,... now fixed.

demo2.v
@@ -76,17 +76,31 @@ pred join o:@classname, o:@classname, o:@classname.
 
 %%%%% Factories %%%%%%%%%%%%%%%%%%%%%%%%%%%%%%%%%%%%%%%%%%%%%%%%%%%%%%%%%%%
 % TODO: document
-% [from LMN FN MN (mtrm ML F)] invariant: "F : forall T LMN, FN T .. -> MN T .." where
-% .. is a sub list of LMN
-pred from o:@factoryname, o:@mixinname, o:mterm.
+% [from FN MN F] invariant:
+% "F : forall T LMN, FN T .. -> MN T .." where
+%  - .. is a sub list of LMN
+% - [factory-requires FN LMN]
+pred from o:@factoryname, o:@mixinname, o:term.
 
 % factory, generated mixin, mean, eg mean : factory -> mixin
 pred extract-mix i:prop, o:@mixinname.
 extract-mix (from _ X _) X.
 
+% [factory-requires F ML] states that the factory ML
+% requires instances of ML to provide new mixins
+pred factory-requires o:@factoryname, o:list @mixinname.
+
+% [factory->mterm Src Tgt MF] provides a mterm to transform
+% Src into Tgt.
+pred factory->mterm i:gref, i:@mixinname, o:mterm.
+factory->mterm Src Tgt (mtrm ML F) :- !,
+  from Src Tgt F, !, factory-requires Src ML.
+
+% [factory-provides F ML] states that the factory ML
+% provides instances of ML
 pred factory-provides i:@factoryname, o:list @mixinname.
 factory-provides Factory ML :- std.do! [
-  std.findall (from Factory T_ MF_) All,
+  std.findall (from Factory T_ F_) All,
   std.map All extract-mix ML,
 ].
 
@@ -218,7 +232,9 @@ subst-mfun Xs (mtrm ML F) (mtrm ML FXs) :- subst-fun Xs F FXs.
 % thus instanciating an abstraction on mixin M_i with X_i
 pred msubst i:term, i:@mixinname, i:term, o:term.
 msubst T M (fun _ Tm F) (F X) :-
-  safe-dest-app Tm (global M) _, !, mixin-for T M X, !.
+  safe-dest-app Tm (global TmGR) _,
+  factory-alias TmGR M, !,
+  mixin-for T M X, !.
 msubst T M (fun N T F) (fun N T FX) :- !, pi m\ msubst T M (F m) (FX m).
 msubst _ _ F F.
 
@@ -238,6 +254,10 @@ msubsts T (mtrm ML F) SFX :- std.do![
 % an instance of the mixin [M T ...], directly or through a factory.
 pred mixin-src o:term, o:@mixinname, o:term.
 
+% [factory-alias Alias Factory]
+% Stores all the aliases factories
+pred factory-alias o:gref, o:gref.
+
 % [mixin-srcs T X MSL] states that MSL is a list of [mixin-src T m X]
 % where m ranges all the mixins that the factory Src can provide,
 % where Src is the type of X.
@@ -245,7 +265,8 @@ pred mixin-srcs i:term, i:term, o:list prop.
 mixin-srcs T X MSL :- std.do! [
   coq.typecheck X XTy,
   term->gr XTy Src,
-  factory-provides Src ML,
+  factory-alias Src Factory,
+  factory-provides Factory ML,
   std.map ML (m\r\ r = mixin-src T m X) MSL
 ].
 
@@ -255,8 +276,9 @@ pred mixin-for o:term, o:@mixinname, o:term.
 mixin-for T M MI :- mixin-src T M Tm, !, std.do! [
   coq.typecheck Tm Ty,
   term->gr Ty Src,
-  if (M = Src) (MI = Tm) (
-      from Src M MF,
+  factory-alias Src Factory,
+  if (M = Factory) (MI = Tm) (
+      factory->mterm Src M MF,
       msubsts T MF F,
       subst-fun [Tm] F MI
   )
@@ -303,7 +325,8 @@ ty-deps (prod N S R) ML' :- !,
   @pi-decl N S x\
     ty-deps (R x) ML,
     safe-dest-app S HD _,
-    if (HD = global GR, mixin-deps GR _) (ML' = [GR|ML]) (ML' = ML).
+    if (HD = global GR, mixin-deps GR _, factory-alias GR F)
+      (ML' = [F|ML]) (ML' = ML).
 ty-deps Ty ML :- whd1 Ty Ty1, !, ty-deps Ty1 ML.
 ty-deps _Ty [].
 
@@ -317,21 +340,21 @@ term-deps T ML :- coq.typecheck T Ty, ty-deps Ty ML.
 pred gr-deps i:gref, o:list @mixinname.
 gr-deps GR ML :- term-deps (global GR) ML.
 
-% [find-all-classes Mixins Classes] states that Classes is a list of classes
+% [find-max-classes Mixins Classes] states that Classes is a list of classes
 %   which contain all the mixins in Mixins.
 % Although it is not strictly necessary, but desirable for debugging,
 % we use a heuristic that tries to minimize the number
 % of classes by assuming Mixins are reversed topologically sorted.
-pred find-all-classes i:list @mixinname, o:list @classname.
-find-all-classes [] [].
-find-all-classes [M|Mixins] [C|Classes] :-
+pred find-max-classes i:list @mixinname, o:list @classname.
+find-max-classes [] [].
+find-max-classes [M|Mixins] [C|Classes] :-
   mixin-first-class M C,
   std.do! [
     class-def (class C _ ML),
     std.filter Mixins (x\ not (std.mem! ML x)) Mixins',
-    find-all-classes Mixins' Classes
+    find-max-classes Mixins' Classes
   ].
-find-all-classes [_|_] _ :- std.fatal-error "cannot find class for mixin".
+find-max-classes [_|_] _ :- std.fatal-error "cannot find class for mixin".
 
 % [under-mixins T ML Pred F] states that F has type
 % fun (m_0 : M_0 T) .. (m_n : M_n T m_i0 .. m_ik) => Body m_0 .. m_n
@@ -383,21 +406,23 @@ mk-phant-abbrev.term K F [unify-arg|AL] K' FAbbrev :- !,
 
 pred mk-phant-abbrev i:string, i:phant-term, o:@constant.
 mk-phant-abbrev N (phant-trm AL T) C :- std.do! [
-  coq.typecheck T _TyT,
   NC is "phant_" ^ N,
+  coq.typecheck T _TTy,
   coq.env.add-const NC T _ ff ff C,
   mk-phant-abbrev.term 0 (global (const C)) AL NParams Abbrev,
   coq.notation.add-abbreviation N NParams Abbrev tt ff
 ].
 
-% [acc-phant-axioms GR] makes a phantom abbreviation for F
-pred acc-phant-axioms i:gref.
-acc-phant-axioms GR :-
+% [acc-factory-aliases GR] makes a phantom abbreviation for F
+pred acc-factory-aliases i:gref, o:list prop.
+acc-factory-aliases GR [] :- factory-alias GR _, !.
+acc-factory-aliases GR Aliases :-
   mk-phant-mixins (global GR) PhGR,
   PhantAbbrevName is {gref->modname GR} ^ "_axioms",
   mk-phant-abbrev PhantAbbrevName PhGR PhC,
-  acc execution-site
-    (clause _ _ (phant-abbrev GR (const PhC) PhantAbbrevName)).
+  acc execution-site (clause _ _ (phant-abbrev GR PhantAbbrevName)),
+  Aliases = [factory-alias GR GR, factory-alias (const PhC) GR],
+  std.forall Aliases a\ acc execution-site (clause _ _ a).
 
 % [mk-phant-unify X1 X2 PF PUF] states that PUF is a phant-term that
 % is starts with unifing X1 and X2 and then outputs PF.
@@ -419,7 +444,8 @@ mk-phant-struct T SI PF (phant-trm [implicit-arg, unify-arg|AL] UF) :-
   get-structure-sort-projection SI Sort,
   pi s\ PF s = phant-trm AL (F s),
   UF = {{fun (s : lp:SI) (u : lib:hb.unify lp:T (lp:Sort s)
-    (lib:hb.none (* "is not canonically a"%string, lp:SI *))) => lp:(F s)}}.
+    (lib:hb.some (lib:hb.pair "is not canonically a"%string lp:SI)))
+      => lp:(F s)}}.
 
 % [mk-phant-struct T CN PF PCF] states that PSF is a phant-term
 % which postulate a structure [s : SI] such that [T = sort s]
@@ -468,17 +494,17 @@ mk-phant-mixins F (phant-trm [real-arg T|AL] (fun T _ CFML)) :- std.do! [
 %  toposort-mixins ML MLSorted,
   ML = MLSorted, % Assumes we give them already sorted in dep order.
   std.rev MLSorted MLSortedRev,
-  find-all-classes MLSortedRev CNL,
+  find-max-classes MLSortedRev CNL,
   (@pi-decl T {{Type}} t\ sigma FML PML\
     std.fold CNL (phant-trm [] {subst-fun [t] EtaF}) (mk-phant-mixins.class t)
       (phant-trm AL (CFML t)))
 ].
 
 % Database for abbreviatation of terms applied to mixins
-% [phant-abbrev Original PhantCst PhantAbbrev]
+% [phant-abbrev Original PhantAbbrev]
 % states that there is an abbreviation /à la/ *pack* for Original,
 % that it is called PhantAbbrev and the underlying constant is PhantCst.
-pred phant-abbrev o:gref, o:gref, o:string.
+pred phant-abbrev o:gref, o:string.
 
 
 % Given a type T, a list of class definition
@@ -537,7 +563,7 @@ mk-id T [A|AS] M (fun `a` AL R) :- std.do! [
 main [str S] :- !, std.do! [
   coq.locate S M,
   % make and register phant-abbrev
-  acc-phant-axioms M,
+  acc-factory-aliases M _,
   % register mixin
   coq.env.typeof-gr M Ty,
   ty-deps Ty ML,
@@ -546,9 +572,10 @@ main [str S] :- !, std.do! [
   Ty = prod T TTy _,
   ID = (fun T TTy t\ {mk-id t ML {mk-app (global M) [t]} }),
   coq.typecheck ID _TyID,
-  FName is {gref->modname M} ^ "_factory",
+  FName is {gref->modname M} ^ "_id_factory",
   coq.env.add-const FName ID _TyID ff ff _CID,
-  acc execution-site (clause _ _ (from M M (mtrm ML ID))),
+  acc execution-site (clause _ _ (factory-requires M ML)),
+  acc execution-site (clause _ _ (from M M ID)),
 ].
 main _ :- coq.error "Usage: declare_mixin <mixin>".
 
@@ -580,6 +607,8 @@ Elpi Typecheck.
   - mixin mn depends on mixins dn
   - all structures that can be generated out of the mixins are declared
     as canonical
+
+% TODO perform a check that the declarations are closed under dependencies
 
 *)
 
@@ -619,9 +648,32 @@ Elpi Typecheck.
 (* %%%%%%%%%%%%%%%%%%%%%%%%%%%%%%%%%%%%%%%%%%%%%%%%%%%%%%%%%%%%%%%%%%%%%% *)
 (* %%%%%%%%%%%%%%%%%%%%%%%%%%%%%%%%%%%%%%%%%%%%%%%%%%%%%%%%%%%%%%%%%%%%%% *)
 
+(** This command declares what a factory reuires.
+% TODO perform a check that the requirements are closed under dependencies
+*)
+
+Elpi Command factory_requires.
+Elpi Accumulate Db hierarchy.db.
+Elpi Accumulate lp:{{
+main [str S|FS] :- !, std.do! [
+  coq.locate S GR,
+  std.map FS locate-string-argument GRFS,
+  factories-provide-mixins GRFS ML _,
+  acc current (clause _ _ (factory-requires GR ML)),
+  acc-factory-aliases GR _,
+].
+main _ :- coq.error "Usage: factory_requires <Factories>..".
+
+}}.
+Elpi Typecheck.
+
 (** This command declares a factory.
 
 TODO : docment
+
+% TODO: check that declare_factory can declare only function that
+% - require elements from {factory_requires} and
+% - provide elements not from {factory_requires}
 
 *)
 
@@ -641,10 +693,10 @@ gather-last-product End (some Last) LastGR EndGR :-
 
 pred factory-comp i:term, i:list @mixinname, i:gref, i:term, i:gref, i:gref, o:term.
 factory-comp T ML Src FF Mid Tgt (fun `src` SrcTy GoF) :- std.do![
-  from Mid Tgt MG,
+  factory->mterm Mid Tgt MG,
   msubsts T (mtrm ML (global Src)) SrcTy,
   @pi-decl `src` SrcTy src\ sigma MSL G F\
-    mixin-srcs T src MSL,
+    mixin-srcs T src MSL, !,
     MSL => (std.do! [
       msubsts T MG G,
       msubsts T (mtrm ML FF) F,
@@ -654,30 +706,30 @@ factory-comp T ML Src FF Mid Tgt (fun `src` SrcTy GoF) :- std.do![
 
 % [declare-factory-from ML Src F Mid Tgt FromI FromO]
 % declares a factory by composing F and G.
-pred declare-factory-from i:list @mixinname, i:gref, i:term,
-  i:gref, i:gref, i:list prop, o:list prop.
-declare-factory-from ML Src F Mid Tgt FromI [NewFrom|FromI] :- FromI => std.do! [
+pred declare-factory-from
+  i:gref, i:term, i:gref, i:gref, i:list prop, o:list prop.
+declare-factory-from Src F Mid Tgt FromI [NewFrom|FromI] :- FromI => std.do! [
+  factory-requires Src ML,
   (@pi-decl `T` {{Type}} t\ sigma MLSrc\
-    under-mixins t ML (factory-comp t ML Src F Mid Tgt) (GoFt t)
+    under-mixins t ML (x\ (factory-comp t ML Src F Mid Tgt x)) (GoFt t)
   ),
   GoF = fun `T` {{Type}} GoFt,
   coq.typecheck GoF GoFTy_,
   Name is {gref->modname Src} ^ "_to_" ^ {gref->modname Tgt},
   coq.env.add-const Name GoF _ ff ff GoFC,
-  NewFrom = from Src Tgt (mtrm ML (global (const GoFC))),
+  NewFrom = from Src Tgt (global (const GoFC)),
   acc execution-site (clause _ _ NewFrom)
 ].
 
 main [str S] :- !, std.do! [
   coq.locate S F,
   coq.env.typeof-gr F Ty,
-  gather-last-product Ty none Src Mid,
-  % declare phantom notation
-  if (not (phant-abbrev Src _ _)) (acc-phant-axioms Src) true,
-  % make the factory
-  ty-deps Ty ML,
-  factory-provides Mid Tgts,
-  std.fold Tgts [] (declare-factory-from ML Src (global F) Mid) _PO
+  gather-last-product Ty none Src MidAlias,
+  factory-alias MidAlias Mid,
+  std.do! [
+    factory-provides Mid Tgts,
+    std.fold Tgts [] (declare-factory-from Src (global F) Mid) _PO
+  ]
 ].
 main _ :- coq.error "Usage: declare_factory <FactoryFunction>".
 
@@ -691,8 +743,6 @@ Elpi Typecheck.
 (** This command declares all the canonical instances the given factories
     provides.
 
-TODO : factor code with declare_context
-
 *)
 
 Elpi Command canonical_instance.
@@ -700,7 +750,6 @@ Elpi Accumulate Db hierarchy.db.
 
 Elpi Accumulate lp:{{
 
-pred factory-instance-for i:@factoryname, o:term.
 main [TS|Args] :- !, std.do! [
   locate-term-argument TS T,
   std.map Args locate-term-argument FIL,
@@ -795,9 +844,9 @@ pred export-operations.aux i:term, i:term, i:term, i:@factoryname, i:list @mixin
 export-operations.aux _ _ _ _ [].
 export-operations.aux Struct ProjSort ProjClass ClassName [indt M|ML] :- !, std.do! [
   Mixin = indt M,
-  from ClassName Mixin (mtrm _ ProjMixin),
+  from ClassName Mixin ProjMixin,
   mixin-deps Mixin Deps,
-  std.map Deps (x\y\ sigma tmp\ from ClassName x (mtrm tmp y)) PDeps,
+  std.map Deps (from ClassName) PDeps,
   coq.CS.canonical-projections M Poperations,
   std.forall Poperations
     (export-1-operation Struct ProjSort ProjClass ProjMixin PDeps),
@@ -825,7 +874,7 @@ declare-coercion SortProjection ClassProjection
   CName is ModNameF ^ "_class_to_" ^ ModNameT ^ "_class",
   SName is ModNameF ^ "_to_" ^ ModNameT,
 
-  std.map TML (x\y\ sigma tmp\ from FC x (mtrm tmp y)) FC2TML,
+  std.map TML (from FC) FC2TML,
   get-class-constructor TC KC,
   Class = global FC,
   (pi T c\ sigma Mixes\
@@ -926,7 +975,7 @@ declare-class ML (indt ClassName) Factories :- std.do! [
   coq.CS.canonical-projections ClassName Projs,
   std.map2 ML Projs (m\ p\ r\ sigma P\
     p = some P,
-    r = from (indt ClassName) m (mtrm [] (global (const P)))) Factories,
+    r = from (indt ClassName) m (global (const P))) Factories,
 ].
 
 % Builds the package record
@@ -980,6 +1029,7 @@ main [str Module|FS] :- !, std.do! [
     acc current (clause _ _ (mixin-first-class m ClassName))),
 
   std.forall Factories (f\ acc current (clause _ _ f)),
+  acc current (clause _ _ (factory-requires (ClassName) [])),
 
   std.forall NewJoins (j\acc current (clause _ _ j)),
 
@@ -1221,6 +1271,7 @@ Definition to_RING_of_AG : RING_of_AG_axioms A :=
 
 End Factories. End S. End RING_of_ASG.
 
+Elpi factory_requires RING_of_ASG.axioms ASG_of_TYPE.axioms.
 Elpi declare_factory RING_of_ASG.to_AG_of_ASG.
 Elpi declare_factory RING_of_ASG.to_RING_of_AG.
 
@@ -1334,55 +1385,46 @@ Module RING_of_AG. Section S.
  Fail Goal AG_of_ASG_axioms A. (* Failure with error message *)
 
  Elpi declare_context A ASG_of_TYPE.axioms AG_of_ASG.axioms.
-
+ Print AG_of_ASG_axioms.
  Goal AG_of_ASG_axioms A. Abort. (* Success of mk-phant-mixin *)
 
  Record axioms := Axioms {
   one : A;
   mul : A -> A -> A;
-  _ : associative mul;
-  _ : left_id one mul;
-  _ : right_id one mul;
-  _ : left_distributive mul add;
-  _ : right_distributive mul add;
+  mulrA : associative mul;
+  mulr1 : left_id one mul;
+  mul1r : right_id one mul;
+  mulrDl : left_distributive mul add;
+  mulrDr : right_distributive mul add;
   }.
 
-Section SRIG_of_ASG.
+Section Factories.
+Variable (a : axioms).
 
-Variables
-  (mul : A -> A -> A)
-  (mulrDl : left_distributive mul add) (mulrDr : right_distributive mul add).
-
-Lemma mul0r : left_zero zero mul.
+Lemma mul0r : left_zero zero (mul a).
 Proof.
-move=> x.
-rewrite -[LHS]add0r addrC.
-rewrite -{2}(addNr (mul x x)) (addrC (opp _)) addrA.
+move=> x; rewrite -[LHS]add0r addrC.
+rewrite -{2}(addNr (mul a x x)) (addrC (opp _)) addrA.
 by rewrite -mulrDl add0r addrC addNr.
 Qed.
 
-Lemma mulr0 : right_zero zero mul.
+Lemma mulr0 : right_zero zero (mul a).
 Proof.
-move=> x.
-rewrite -[LHS]add0r addrC.
-rewrite -{2}(addNr (mul x x)) (addrC (opp _)) addrA.
+move=> x; rewrite -[LHS]add0r addrC.
+rewrite -{2}(addNr (mul a x x)) (addrC (opp _)) addrA.
 by rewrite -mulrDr add0r addrC addNr.
 Qed.
 
-End SRIG_of_ASG.
-
-Section Factories.
-Variable a : axioms.
-
 Check SRIG_of_ASG.Axioms.
 Definition to_SRIG_of_ASG : SRIG_of_ASG_axioms A :=
-  let: Axioms one mul mulA mul1x mulx1 mulDl mulDr := a in
-  @SRIG_of_ASG.Axioms A _ one mul mulA mul1x mulx1 mulDl mulDr
-                      (mul0r _ mulDl) (mulr0 _ mulDr).
+  @SRIG_of_ASG.Axioms A _ (one a) (mul a) (mulrA a) (mulr1 a) (mul1r a)
+     (mulrDl a) (mulrDr a) (mul0r) (mulr0).
 
 End Factories. End S. End RING_of_AG.
-Elpi Print debug.
+
 Check RING_of_AG.to_SRIG_of_ASG.
+
+Elpi factory_requires RING_of_AG.axioms ASG_of_TYPE.axioms AG_of_ASG.axioms.
 Elpi declare_factory RING_of_AG.to_SRIG_of_ASG.
 
 (* To not break clients / provide shortcuts for users not interested in the
@@ -1419,7 +1461,245 @@ Definition to_RING_of_AG : RING_of_AG_axioms A :=
 
 End Factories. End S. End RING_of_ASG.
 
+Elpi factory_requires RING_of_ASG.axioms ASG_of_TYPE.axioms.
 Elpi declare_factory RING_of_ASG.to_AG_of_ASG.
 Elpi declare_factory RING_of_ASG.to_RING_of_AG.
 
 End Example3.
+
+
+(******************************************************************************)
+(* Example 4                                                                  *)
+(******************************************************************************)
+
+Module Example4.
+
+Elpi declare_structure "TYPE".
+Import TYPE.Exports.
+
+Module SG_of_TYPE. Section S.
+ Variable S : Type.
+ Elpi declare_context S.
+ (* Check (eq_refl _ : TYPE.sort _ = S). *)
+ Record axioms := Axioms {
+  zero : S;
+  add : S -> S -> S;
+  _ : associative add;
+  _ : left_id zero add;
+  _ : right_id zero add;
+  }.
+End S. End SG_of_TYPE.
+
+Elpi declare_mixin SG_of_TYPE.axioms.
+Elpi declare_structure "SG" SG_of_TYPE.axioms.
+Import SG.Exports.
+
+Lemma addrA {A : SG.type} : associative (@add A).
+Proof. by case: A => ? [[]]. Qed.
+
+Lemma add0r {A : SG.type} : left_id (@zero A) add.
+Proof. by case: A => ? [[]]. Qed.
+
+Lemma addr0 {A : SG.type} : right_id (@zero A) add.
+Proof. by case: A => ? [[]]. Qed.
+
+Module ASG_of_SG. Section S.
+ Variable A : Type.
+ Elpi declare_context A SG_of_TYPE.axioms.
+ (* Check (eq_refl _ : TYPE.sort _ = A). *)
+ Record axioms := Axioms {
+  _ : commutative (add : A -> A -> A);
+  }.
+End S. End ASG_of_SG.
+
+Elpi declare_mixin ASG_of_SG.axioms.
+
+Elpi declare_structure "ASG" SG.class_of ASG_of_SG.axioms.
+Import ASG.Exports.
+
+Lemma addrC {A : ASG.type} : commutative (@add A).
+Proof. by case: A => ? [[? ? ? ? ?] []]. Qed.
+
+Module ASG_of_TYPE. Section S.
+ Variable A : Type.
+ Elpi declare_context A.
+ (* Check (eq_refl _ : TYPE.sort _ = A). *)
+ Record axioms := Axioms {
+  zero : A;
+  add : A -> A -> A;
+  addA : associative add;
+  addC : commutative add;
+  addr0 : left_id zero add;
+  }.
+
+  Section Factories.
+  Variable (a : axioms).
+
+  Fact add0r : right_id (zero a) (add a).
+  Proof. by move=> x; rewrite addC addr0. Qed.
+
+  Definition to_SG_of_TYPE : SG_of_TYPE_axioms A :=
+    SG_of_TYPE.Axioms _ (zero a) (add a) (addA a) (addr0 a) add0r.
+  Elpi canonical_instance A to_SG_of_TYPE.
+
+  Definition to_ASG_of_SG : ASG_of_SG_axioms A :=
+    ASG_of_SG.Axioms _ _ (addC a : commutative SG.Exports.add).
+  Elpi canonical_instance A to_ASG_of_SG.
+
+  End Factories.
+End S. End ASG_of_TYPE.
+
+Elpi factory_requires ASG_of_TYPE.axioms.
+Elpi declare_factory ASG_of_TYPE.to_SG_of_TYPE.
+Elpi declare_factory ASG_of_TYPE.to_ASG_of_SG.
+
+Module AG_of_ASG. Section S.
+ Variable A : Type.
+ Elpi declare_context A ASG_of_TYPE.axioms.
+ Record axioms := Axioms {
+  opp : A -> A;
+  _ : left_inverse zero opp add;
+  }.
+End S. End AG_of_ASG.
+
+Elpi declare_mixin AG_of_ASG.axioms.
+
+Elpi declare_structure "AG" ASG_of_TYPE.axioms AG_of_ASG.axioms.
+Import AG.Exports.
+
+Print Module AG.Exports.
+
+Check opp zero.
+
+Lemma addNr {A : AG.type} : left_inverse (@zero A) opp add.
+Proof. by case: A => ? [? []]. Qed.
+
+Module SRIG_of_ASG. Section S.
+ Variable A : Type.
+ Elpi declare_context A ASG_of_TYPE.axioms.
+ Record axioms := Axioms {
+  one : A;
+  mul : A -> A -> A;
+  _ : associative mul;
+  _ : left_id one mul;
+  _ : right_id one mul;
+  _ : left_distributive mul add;
+  _ : right_distributive mul add;
+  _ : left_zero zero mul;
+  _ : right_zero zero mul;
+  }.
+End S. End SRIG_of_ASG.
+
+Elpi declare_mixin SRIG_of_ASG.axioms.
+
+Elpi declare_structure "SRIG" ASG_of_TYPE.axioms SRIG_of_ASG.axioms.
+Import SRIG.Exports.
+
+Elpi declare_structure "RING" ASG_of_TYPE.axioms AG_of_ASG.axioms SRIG_of_ASG.axioms.
+Import RING.Exports.
+
+Check opp zero. (* ASG.sort _ = AG.sort _ *)
+Check add zero one. (* ASG.sort _ = SRIG.sort _ *)
+Check opp one. (* AG.sort _ = SRIG.sort _ *)
+
+Lemma mulrA {A : SRIG.type} : associative (@mul A).
+Proof. by case: A => ? [? []]. Qed.
+Lemma mul1r {A : SRIG.type} : left_id (@one A) mul.
+Proof. by case: A => ? [? []]. Qed.
+Lemma mulr1 {A : SRIG.type} : right_id (@one A) mul.
+Proof. by case: A => ? [? []]. Qed.
+Lemma mulrDl {A : SRIG.type} : left_distributive (@mul A) add.
+Proof. by case: A => ? [? []]. Qed.
+Lemma mulrDr {A : SRIG.type} : right_distributive (@mul A) add.
+Proof. by case: A => ? [? []]. Qed.
+Lemma mul0r {A : SRIG.type} : left_zero (@zero A) mul.
+Proof. by case: A => ? [? []]. Qed.
+Lemma mulr0 {A : SRIG.type} : right_zero (@zero A) mul.
+Proof. by case: A => ? [? []]. Qed.
+
+Module RING_of_AG. Section S.
+ Variable A : Type.
+
+ Fail Goal AG_of_ASG_axioms A. (* Failure with error message *)
+
+ Elpi declare_context A ASG_of_TYPE.axioms AG_of_ASG.axioms.
+
+ Goal AG_of_ASG_axioms A. Abort. (* Success of mk-phant-mixin *)
+
+ Record axioms := Axioms {
+  one : A;
+  mul : A -> A -> A;
+  mulrA : associative mul;
+  mulr1 : left_id one mul;
+  mul1r : right_id one mul;
+  mulrDl : left_distributive mul add;
+  mulrDr : right_distributive mul add;
+  }.
+
+Section Factories.
+Variable (a : axioms).
+
+Lemma mul0r : left_zero zero (mul a).
+Proof.
+move=> x; rewrite -[LHS]add0r addrC.
+rewrite -{2}(addNr (mul a x x)) (addrC (opp _)) addrA.
+by rewrite -mulrDl add0r addrC addNr.
+Qed.
+
+Lemma mulr0 : right_zero zero (mul a).
+Proof.
+move=> x; rewrite -[LHS]add0r addrC.
+rewrite -{2}(addNr (mul a x x)) (addrC (opp _)) addrA.
+by rewrite -mulrDr add0r addrC addNr.
+Qed.
+
+Check SRIG_of_ASG.Axioms.
+Definition to_SRIG_of_ASG : SRIG_of_ASG_axioms A :=
+  @SRIG_of_ASG.Axioms A _ (one a) (mul a) (mulrA a) (mulr1 a) (mul1r a)
+     (mulrDl a) (mulrDr a) (mul0r) (mulr0).
+
+End Factories. End S. End RING_of_AG.
+
+Check RING_of_AG.to_SRIG_of_ASG.
+Elpi factory_requires RING_of_AG.axioms ASG_of_TYPE.axioms AG_of_ASG.axioms.
+Elpi declare_factory RING_of_AG.to_SRIG_of_ASG.
+
+(* To not break clients / provide shortcuts for users not interested in the
+   new AG class. *)
+Module RING_of_ASG. Section S.
+Variable A : Type.
+
+Elpi declare_context A ASG_of_TYPE.axioms.
+
+Record axioms := Axioms {
+  opp : A -> A;
+  one : A;
+  mul : A -> A -> A;
+  _ : left_inverse zero opp add;
+  _ : associative mul;
+  _ : left_id one mul;
+  _ : right_id one mul;
+  _ : left_distributive mul add;
+  _ : right_distributive mul add;
+  }.
+
+Section Factories.
+Variable a : axioms.
+
+Definition to_AG_of_ASG : AG_of_ASG_axioms A :=
+  let: Axioms opp one mul addNr _ _ _ _ _ := a in
+  @AG_of_ASG.Axioms A _ opp addNr.
+
+Elpi canonical_instance A to_AG_of_ASG.
+
+Definition to_RING_of_AG : RING_of_AG_axioms A :=
+  let: Axioms _ _ _ _ mulrA mul1r mulr1 mulrDl mulrDr := a in
+  @RING_of_AG.Axioms A _ _ _ mulrA mul1r mulr1 mulrDl mulrDr.
+
+End Factories. End S. End RING_of_ASG.
+
+Elpi factory_requires RING_of_ASG.axioms ASG_of_TYPE.axioms.
+Elpi declare_factory RING_of_ASG.to_AG_of_ASG.
+Elpi declare_factory RING_of_ASG.to_RING_of_AG.
+
+End Example4.
